src/program_proof/simplefs/inode_proof.v
@@ -1,6 +1,77 @@
 From Perennial.program_proof Require Import proof_prelude.
+From Goose.github_com Require Import tchajed.simplefs.
 From Goose.github_com Require Import tchajed.simplefs.inode.
 
 From Perennial.program_proof Require Import disk_prelude.
 From Perennial.program_proof Require Import marshal_stateless_proof.
 From Perennial.goose_lang.lib Require Import typed_slice.
+
+Set Default Proof Using "Type".
+
+Module inodeType.
+Inductive t :=
+| invalid
+| dirType
+| fileType.
+
+Definition rep (x: t) : w32 :=
+  W32 (match x with
+  | invalid => 0
+  | dirType => 1
+  | fileType => 2
+  end).
+
+Definition is_valid (v: w32) :=
+  0 < uint.Z v < 3.
+
+End inodeType.
+
+Section proof.
+Context `{!heapGS Σ}.
+
+Theorem wp_InodeType__IsValid (v: w32) :
+  {{{ True }}}
+    InodeType__IsValid #v
+  {{{ RET #(bool_decide (inodeType.is_valid v)); True }}}.
+Proof.
+  (*@ func (t InodeType) IsValid() bool {                                     @*)
+  (*@     return t != Invalid && t <= FileType                                @*)
+  (*@ }                                                                       @*)
+  iIntros (Φ) "Hpre HΦ".
+  wp_rec. wp_pures.
+  iDestruct ("HΦ" with "[//]") as "HΦ".
+  destruct_decide (bool_decide_reflect (#v = #(W32 0))) as Heq.
+  - rewrite /=; wp_pures. iModIntro.
+    iExactEq "HΦ".
+    rewrite bool_decide_eq_false_2 //.
+    inv Heq.
+    rewrite /inodeType.is_valid. word.
+  - rewrite /=; wp_pures. iModIntro.
+    iExactEq "HΦ".
+    repeat f_equal.
+    apply bool_decide_ext.
+    rewrite /inodeType.is_valid.
+    cut (uint.Z v ≠ 0); [ word | ].
+    { intros H.
+      contradiction Heq.
+      repeat f_equal.
+      word. }
+Qed.
+
+End proof.
+
+Module inode_rep.
+Record t := {
+    typ: inodeType.t;
+    len: w64;
+    meta: w32; (* a meta ia just a w32 mode for simplicity *)
+    block_ptrs: vec w32 28;
+}.
+
+Section proof.
+Context `{!heapGS Σ}.
+
+Definition is_meta (v: val) (meta: w32) :=
+  v = (#meta, #())%V.
+
+End proof.
